MyLean/MyDataStructures/Stack.lean
@@ -4,132 +4,514 @@ import Mathlib.Tactic.TypeStar
 import Mathlib.Data.Nat.Notation
 import Mathlib.Tactic.Use
 import Mathlib.Tactic.ApplyAt
+import Mathlib.Tactic.NthRewrite
+import Mathlib.Tactic.Contrapose
 
 inductive Stack (α : Type*) where
-  | empty  : Stack α
-  | push : α → Stack α → Stack α
+  | empty : Stack α
+  | push  : α → Stack α → Stack α
 
 namespace Stack
 
+-- Definitions
+
 protected def toString {α : Type*} [ToString α] (t : Stack α) : String :=
   match t with
-  | empty => ""
+  | empty     => ""
   | push a as => toString a ++ " " ++ Stack.toString as
 
 instance {α : Type*} [ToString α] : ToString (Stack α) where
   toString := Stack.toString
 
-def pop {α : Type*} : Stack α → Option (α × Stack α)
-  | empty => none
-  | push a s => some (a, s)
 
-def rev_append {α : Type*} : Stack α → Stack α → Stack α
-| empty, s2 => s2
-| push a s1, s2 => rev_append s1 (push a s2)
+def pop {α : Type*} : Stack α → (Option α) × Stack α
+  | empty    => (none, empty)
+  | push a s => (some a, s)
 
-def reverse {α : Type*} (s : Stack α) :=
-  rev_append s empty
 
-def append {α : Type*} (s1 s2 : Stack α) :=
-  rev_append (reverse s1) s2
+def app {α : Type*} : Stack α → Stack α → Stack α
+| empty, t    => t
+| push a s, t => push a (app s t)
 
-def nonempty_eq_push {α : Type*} (s : Stack α) :
-s ≠ (empty : Stack α) → ∃ (a : α) (t : Stack α), s = push a t := by
-  intro h1
-  cases h2 : s with
-  | empty =>
-    tauto
-  | push a as =>
-    use a, as
+-- ptb = push to bottom
+def ptb {α : Type*} : α → Stack α → Stack α
+| a, empty    => push a empty
+| a, push b s => push b (ptb a s)
 
-theorem reverse_pushAux {α : Type*} (as : Stack α) :
-∀ (b : α) (bs : Stack α), rev_append as (push b bs) ≠ empty := by
-  induction as with
-  | empty =>
-    intro b bs
-    rw [rev_append]
-    tauto
-  | push a as ih =>
-    intro b bs
-    rw [rev_append]
-    specialize ih a (push b bs)
-    exact ih
+def rev {α : Type*} : Stack α → Stack α
+| empty    => empty
+| push a s => ptb a (rev s)
 
-theorem reverse_push {α : Type*} (a : α) (as : Stack α) :
-∃ (b : α) (bs : Stack α), reverse (push a as) = push b bs := by
-  have : (push a as).reverse ≠ empty := by
-    apply reverse_pushAux
-  apply nonempty_eq_push at this
-  rcases this with ⟨b, bs, this⟩
-  use b, bs
+def size {α : Type*} : Stack α → ℕ
+| empty    => 0
+| push _ s => size s + 1
+
+def ind {α : Type*} : ℕ → Stack α → Option α
+-- ind n s = the nth entry of the Stack s, or none
+| _    , empty    => none
+| 0    , push a _ => some a
+| n + 1, push _ s => ind n s
+
+def app_rev {α : Type*} : Stack α → Stack α → Stack α
+| empty, t    => t
+| push a s, t => app_rev s (push a t)
 
 def list_to_stack {α : Type*} : List α → Stack α
-  | []      => empty
-  | a :: as => push a (list_to_stack as)
+| []      => empty
+| a :: as => push a (list_to_stack as)
 
-def combine {α : Type*} : Stack α → Stack α → Stack α
-  | empty, t    => t
-  | push a s, t => push a (combine s t)
+/- Functions defined below are tail-recursive variants
+of functions defined above-/
+
+def rev_tr {α : Type*} (s : Stack α) := app_rev s empty
+
+def app_tr {α : Type*} (s1 s2 : Stack α) :=
+  app_rev (rev_tr s1) s2
+
+def size_tr {α : Type*} (s : Stack α) :=
+  let rec aux : ℕ → Stack α → ℕ
+    | acc, empty    => acc
+    | acc, push _ s => aux (acc + 1) s
+  aux 0 s
+
+----------------------------------------
+-- Equality with tail-recursive variants
+
+theorem app_ptb_left {α : Type*} (a : α) (s t : Stack α) :
+(ptb a s).app t = s.app (push a t) := by
+  induction s with
+  | empty =>
+    rw [ptb, app, app, app]
+  | push b s ih =>
+    rw [ptb, app, ih, app]
+
+theorem app_ptb_right {α : Type*} (a : α) (s t : Stack α) :
+s.app (ptb a t) = ptb a (s.app t) := by
+  induction s with
+  | empty =>
+    rw [app, app]
+  | push b s ih =>
+    rw [app, app, ptb, ih]
+
+theorem app_rev_ptb_left {α : Type*}
+(a : α) (s t : Stack α) :
+app_rev (ptb a s) t = push a (app_rev s t) := by
+  induction s generalizing t with
+  | empty =>
+    rw [ptb, app_rev, app_rev, app_rev]
+  | push b s ih =>
+    rw [ptb, app_rev, app_rev]
+    exact ih (push b t)
+
+theorem app_rev_ptb_right {α : Type*}
+(a : α) (s t : Stack α) :
+app_rev s (ptb a t) = ptb a (app_rev s t) := by
+  induction s generalizing t with
+  | empty =>
+    rw [app_rev, app_rev]
+  | push b s ih =>
+    rw [app_rev, app_rev, ← ptb]
+    exact ih (push b t)
+
+theorem app_rev_eq {α : Type*} (s t : Stack α) :
+s.app_rev t = s.rev.app t := by
+  induction s generalizing t with
+  | empty =>
+    rw [app_rev, rev, app]
+  | push b s ih =>
+    rw [app_rev, rev, app_ptb_left]
+    exact ih (push b t)
+
+theorem app_empty {α : Type*} (s : Stack α) :
+s.app empty = s := by
+  induction s with
+  | empty =>
+    rw [app]
+  | push a s ih =>
+    rw [app, ih]
+
+theorem rev_eq {α : Type*} (s : Stack α) :
+s.rev_tr = s.rev := by
+  have := app_rev_eq s empty
+  rw [app_empty, ← rev_tr] at this
+  exact this
+
+theorem rev_ptb {α : Type*} (a : α) (s : Stack α) :
+(ptb a s).rev = push a s.rev := by
+  rw [← rev_eq, rev_tr, app_rev_ptb_left, ← rev_tr, rev_eq]
+
+theorem rev_rev {α : Type*} (s : Stack α) :
+s.rev.rev = s := by
+  induction s with
+  | empty =>
+    rw [rev, rev]
+  | push a s ih =>
+    rw [rev, rev_ptb, ih]
+
+theorem app_eq {α : Type*} (s t : Stack α) :
+s.app_tr t = s.app t := by
+  rw [app_tr, app_rev_eq, rev_eq, rev_rev]
+
+----------------------
+-- Theorems about size
+
+theorem size_aux_succ {α : Type*} (n : ℕ) (s : Stack α) :
+size_tr.aux (n + 1) s = size_tr.aux n s + 1 := by
+  induction s generalizing n with
+  | empty =>
+    rw [size_tr.aux, size_tr.aux]
+  | push a s ih =>
+    rw [size_tr.aux, size_tr.aux]
+    exact ih (n + 1)
+
+theorem size_eq {α : Type*} (s : Stack α) :
+s.size_tr = s.size := by
+  induction s with
+  | empty =>
+    rw [size_tr, size_tr.aux, size]
+  | push a s ih =>
+    rw [size_tr, size_tr.aux, size_aux_succ, ← size_tr,
+        size, ih]
+
+theorem size_of_single {α : Type*} (a : α) :
+size (push a empty) = 1 := by
+  rw [size, size, Nat.zero_add]
+
+theorem size_eq_zero_iff_empty {α : Type*} (s : Stack α) :
+size s = 0 ↔ s = empty := by
+  cases s with
+  | empty =>
+    rw [size]
+    simp only
+  | push a s =>
+    rw [size]
+    simp only [Nat.add_eq_zero, Nat.succ_ne_self,
+               and_false, reduceCtorEq]
+
+theorem size_of_ptb {α : Type*} (a : α) (s : Stack α) :
+size (ptb a s) = size s + 1 := by
+  induction s with
+  | empty =>
+    rw [ptb, size_of_single, size, Nat.zero_add]
+  | push b s ih =>
+    rw [ptb, size, size, ih]
+
+theorem size_of_rev {α : Type*} (s : Stack α) :
+size s.rev = size s := by
+  induction s with
+  | empty =>
+    rw [rev]
+  | push a s ih =>
+    rw [rev, size_of_ptb, size, ih]
+
+theorem size_of_app {α : Type*} (s t : Stack α) :
+size (s.app t) = size s + size t := by
+  induction s with
+  | empty =>
+    rw [app, size, Nat.zero_add]
+  | push a s ih =>
+    rw [app, size, size, ih, Nat.add_right_comm]
+
+theorem size_of_app_rev {α : Type*} (s t : Stack α) :
+size (s.app_rev t) = size s + size t := by
+  induction s generalizing t with
+  | empty =>
+    rw [app_rev, size, Nat.zero_add]
+  | push a s ih =>
+    rw [app_rev, size]
+    specialize ih (push a t)
+    rw [ih, size]; omega
+
+theorem size_ne_zero_iff_exists_push {α : Type*}
+(s : Stack α) : s.size ≠ 0 ↔
+∃ (a : α) (t : Stack α), s = push a t := by
+  constructor
+  · intro h
+    rw [ne_eq, size_eq_zero_iff_empty] at h
+    cases s with
+    | empty => contradiction
+    | push b s =>
+      use b; use s
+  intro h
+  rcases h with ⟨a, t, h⟩
+  rw [h, size]; omega
+
+theorem size_ne_zero_iff_exists_ptb {α : Type*}
+(s : Stack α) : s.size ≠ 0 ↔
+∃ (a : α) (t : Stack α), s = ptb a t := by
+  induction s with
+  | empty =>
+    rw [size]
+    constructor
+    · tauto
+    intro h
+    rcases h with ⟨a, t, h⟩
+    have : size (empty : Stack α) = size (ptb a t) := by rw [h]
+    rw [size, size_of_ptb] at this
+    omega
+  | push b s ih =>
+    rw [size]
+    constructor
+    · intro h; clear h
+      cases s with
+      | empty =>
+        use b
+        use empty
+        rw [ptb]
+      | push a s =>
+        rcases ih with ⟨h, -⟩
+        rw [size] at h
+        have h2 : s.size + 1 ≠ 0 := by omega
+        apply h at h2
+        rcases h2 with ⟨c, t, h⟩
+        rw [h, ← ptb]
+        use c
+        use push b t
+    omega
+
+theorem exists_push_of_ptb {α : Type*} (a : α) (s : Stack α) :
+∃ (b : α) (t : Stack α), push b t = ptb a s := by
+  have h1 : size (ptb a s) ≠ 0 := by
+    rw [size_of_ptb]; omega
+  rw [size_ne_zero_iff_exists_push] at h1
+  rcases h1 with ⟨b, t, h1⟩
+  use b
+  use t
+  rw [h1]
+
+--------------------------
+-- Theorems about indexing
+
+theorem eq_of_ind_eq {α : Type*} (s t : Stack α)
+(h : ∀ n : ℕ, ind n s = ind n t) : s = t := by
+  induction s generalizing t with
+  | empty =>
+    specialize h 0
+    rw [ind] at h
+    cases t with
+    | empty => rfl
+    | push b t =>
+      rw [ind] at h
+      tauto
+  | push a s ih =>
+    cases t with
+    | empty =>
+      specialize h 0
+      simp only [ind] at h
+      tauto
+    | push b t =>
+      have h2 := h 0
+      simp only [ind, Option.some.injEq] at h2
+      rw [h2]
+      specialize ih t
+      have h3 : ∀ (n : ℕ), ind n s = ind n t := by
+        intro n
+        specialize h (n + 1)
+        rw [ind, ind] at h
+        exact h
+      apply ih at h3
+      rw [h3]
+
+theorem ind_of_sizeAux {α : Type*} (n : ℕ) (s : Stack α)
+(sn : size s = n) :
+ind n s = none := by
+  induction n generalizing s with
+  | zero =>
+    rw [size_eq_zero_iff_empty] at sn
+    rw [sn, ind]
+  | succ n ih =>
+    cases s with
+    | empty =>
+      symm at sn
+      rw [size, Nat.add_eq_zero] at sn
+      tauto
+    | push a s =>
+      rw [size] at sn
+      apply Nat.add_right_cancel at sn
+      rw [ind]
+      exact ih s sn
+
+theorem ind_of_size {α : Type*} (s : Stack α) :
+ind (size s) s = none := by
+  have := ind_of_sizeAux (n := size s) (s := s)
+  tauto
+
+theorem ind_of_lt_size {α : Type*} (n : ℕ) (s : Stack α)
+(sn : n < size s) : ind n s ≠ none := by
+  induction s generalizing n with
+  | empty =>
+    rw [size] at sn; tauto
+  | push a s ih =>
+    rw [size] at sn
+    cases n with
+    | zero =>
+      rw [ind]; tauto
+    | succ n =>
+      simp only [Nat.add_lt_add_iff_right] at sn
+      rw [ind]
+      exact ih n sn
+
+theorem ind_succ_none_of_ind_none {α : Type*}
+(n : ℕ) (s : Stack α) (h : ind n s = none) :
+ind (n + 1) s = none := by
+  induction n generalizing s with
+  | zero =>
+    cases s with
+    | empty =>
+      rw [ind]
+    | push a s =>
+      rw [ind] at h; tauto
+  | succ n ih =>
+    cases s with
+    | empty => rw [ind]
+    | push a s =>
+      rw [ind]
+      rw [ind] at h
+      exact ih s h
+
+theorem ind_of_gt_size {α : Type*} (n : ℕ) (s : Stack α)
+(sn : size s < n) : ind n s = none := by
+  have h1 : ∀ c : ℕ, ind (size s + c) s = none := by
+    intro c
+    induction c generalizing s with
+    | zero =>
+      rw [Nat.add_zero]
+      apply ind_of_size
+    | succ c ih =>
+      rw [← Nat.add_assoc]
+      apply ind_succ_none_of_ind_none
+      exact ih s sn
+  apply Nat.exists_eq_add_of_lt at sn
+  rcases sn with ⟨k, sn⟩
+  rw [sn, Nat.add_assoc]
+  exact h1 (k + 1)
+
+theorem ind_size_of_ptb {α : Type*} (a : α) (s : Stack α) :
+ind (size s) (ptb a s) = a := by
+  induction s with
+  | empty =>
+    rw [size, ptb, ind]
+  | push b s ih =>
+    rw [size, ptb, ind, ih]
+
+theorem ind_lt_size_of_ptb {α : Type*}
+(n : ℕ) (a : α) (s : Stack α) (sn : n < size s) :
+ind n (ptb a s) = ind n s := by
+  induction s generalizing n with
+  | empty =>
+    rw [size] at sn; tauto
+  | push b s ih =>
+    rw [ptb]
+    rw [size] at sn
+    cases n with
+    | zero =>
+      rw [ind, ind]
+    | succ n =>
+      rw [ind, ind]
+      rw [Nat.add_lt_add_iff_right] at sn
+      exact ih n sn
+
+theorem ind_of_rev {α : Type*} (s : Stack α) (n : ℕ)
+(sn : n < size s) : ind n s =
+ind (size s - 1 - n) s.rev := by
+  induction n generalizing s with
+  | zero =>
+    cases s with
+    | empty =>
+      rw [size] at sn; tauto
+    | push a s =>
+      rw [rev, Nat.sub_zero, ind, size, Nat.add_sub_cancel,
+          ← size_of_rev, ind_size_of_ptb]
+  | succ n ih =>
+    cases s with
+    | empty =>
+      rw [size] at sn; tauto
+    | push b s =>
+      rw [size, Nat.add_lt_add_iff_right] at sn
+      have h1 := ih s sn
+      rw [ind, size, Nat.add_sub_cancel, h1, rev,
+          Nat.sub_sub, Nat.add_comm]
+      cases s with
+      | empty =>
+        rw [size] at sn; tauto
+      | push c s =>
+        have h2 : (push c s).size - (n + 1) < (push c s).rev.size := by
+          rw [size_of_rev, size]
+          omega
+        have h3 := ind_lt_size_of_ptb
+          (n := (push c s).size - (n + 1))
+          (a := b) (s := (push c s).rev) h2
+        rw [h3]
+
+theorem ind_app_left {α : Type*} (n : ℕ) (s t : Stack α)
+(sn : n < s.size) : ind n (s.app t) = ind n s := by
+  induction s generalizing n with
+  | empty =>
+    rw [size] at sn; tauto
+  | push a s ih =>
+    rw [size] at sn
+    rw [app]
+    cases n with
+    | zero =>
+      rw [ind, ind]
+    | succ n =>
+      rw [ind, ind]
+      simp only [Nat.add_lt_add_iff_right] at sn
+      exact ih n sn
+
+theorem ind_of_rev' {α : Type*} (n : ℕ) (s : Stack α)
+(h : n < s.size) :
+ind n s.rev = ind (s.size - 1 - n) s := by
+  rw [← size_of_rev] at h
+  have h2 := ind_of_rev (n := n) (s := s.rev) h
+  rw [rev_rev, size_of_rev] at h2
+  exact h2
+
+theorem ind_size_left_of_app {α : Type*} (a : α)
+(s t : Stack α) : ind s.size (s.app (push a t)) = a := by
+  induction s with
+  | empty =>
+    rw [size, app, ind]
+  | push b s ih =>
+    rw [size, app, ind]
+    exact ih
+
+theorem app_rev_exists {α : Type*} (s t : Stack α) :
+∃ r : Stack α, s.app_rev t = r.app t := by
+  induction s generalizing t with
+  | empty =>
+    use empty
+    rw [app_rev, app]
+  | push a s ih =>
+    rw [app_rev]
+    specialize ih (push a t)
+    rcases ih with ⟨q, ih⟩
+    rw [ih]
+    use ptb a q
+    rw [app_ptb_left]
+
+theorem ind_eq_size_of_app_rev {α : Type*}
+(a : α) (s t : Stack α) :
+ind s.size ((push a s).app_rev t) = a := by
+  rw [app_rev]
+  have h1 := app_rev_exists (s := s) (t := push a t)
+  rcases h1 with ⟨r, h1⟩
+  have h2 : s.size = r.size := by
+    have h2 : size (s.app_rev (push a t)) =
+    size (r.app (push a t)) := by
+      rw [h1]
+    rw [size_of_app_rev, size_of_app,
+        Nat.add_right_cancel_iff] at h2
+    exact h2
+  rw [h1, h2, ind_size_left_of_app]
+
+theorem size_of_app_eq_app_rev {α : Type*}
+(r s t : Stack α) (h : r.app t = s.app_rev t) :
+size r = size s := by
+  have h1 :size (r.app t) = size (s.app_rev t) := by
+    rw [h]
+  rw [size_of_app, size_of_app_rev,
+      Nat.add_right_cancel_iff] at h1
+  exact h1
 
 end Stack
-
-structure Queue (α : Type*) where
-  front : Stack α
-  back : Stack α
-
-namespace Queue
-
-protected def toString {α : Type*} [ToString α] (t : Queue α) : String :=
-  "[ " ++ toString t.front ++ "] [ " ++ toString t.back ++ "]"
-
-instance {α : Type*} [ToString α] : ToString (Queue α) where
-  toString := Queue.toString
-
-end Queue
-
-open Stack
-
-def enqueue {α : Type*} (a : α) (q : Queue α) : Queue α where
-  front := q.front
-  back  := push a q.back
-
-def dequeue {α : Type*} (q : Queue α) : ((Option α) × Queue α) :=
-  match q.front with
-  | push a as =>
-    (some a, {front := as
-            , back  := q.back})
-  | empty =>
-    match reverse q.back with
-    | push b bs =>
-      (some b, {front := bs
-              , back  := empty})
-    | empty =>
-      (none, {front := empty
-            , back  := empty})
-
-def Fib (n : ℕ) :=
-  let rec FibAux : ℕ → (ℕ × ℕ) → (ℕ × ℕ)
-    | 0, (a, b) => (a, b)
-    | n + 1, (a, b) => FibAux n (b, a + b)
-  (FibAux n (1, 0)).2
-
-def hi := list_to_stack [1, 6, 2, 3, 8]
-def bye := list_to_stack [4, 4, 5, 1, 3]
-
-def q1 : Queue ℕ := {front := hi
-                   , back  := bye}
-def q2 := (dequeue q1).2
-def q3 := (dequeue q2).2
-def q4 := (dequeue q3).2
-def q5 := (dequeue q4).2
-def q6 := (dequeue q5).2
-def q7 := (dequeue q6).2
-
-#eval hi
-#eval bye
-#eval reverse bye
-#eval combine hi bye
-#eval append hi bye
-#eval q5
-#eval q6
-#eval q7
