MyLean/MyDataStructures/BinTree.lean
@@ -1,0 +1,249 @@
+import MyLean.MyDataStructures.Queue
+import Mathlib.Tactic.Tauto
+import Mathlib.Data.Prod.Basic
+
+set_option linter.unusedVariables false
+
+inductive BinTree (α : Type*) where
+  | empty : BinTree α
+  | node  : α → BinTree α → BinTree α → BinTree α
+
+namespace BinTree
+
+protected def toString {α : Type*} [ToString α] (t : BinTree α) : String :=
+  match t with
+  | empty => ""
+  | node a left right => toString a ++ " ( " ++
+    BinTree.toString left ++
+    " ) ( " ++ BinTree.toString right ++ " )"
+
+instance {α : Type*} [ToString α] : ToString (BinTree α) where
+  toString := BinTree.toString
+
+def size {α : Type*} : BinTree α → ℕ
+  | empty      => 0
+  | node _ left right => 1 + size left + size right
+
+-- Size including empty children
+def size' {α : Type*} : BinTree α → ℕ
+  | empty => 1
+  | node _ left right =>
+    1 + size' left + size' right
+
+-- SBS = Size of BinTree Stack
+def SBS {α : Type*} : Stack (BinTree α) → ℕ
+  | Stack.empty => 0
+  | Stack.push q qs =>
+    size q + SBS qs
+
+def SBS' {α : Type*} : Stack (BinTree α) → ℕ
+  | Stack.empty => 0
+  | Stack.push q qs =>
+    size' q + SBS' qs
+
+-- SBQ = Size of BinTree Queue
+def SBQ {α : Type*} (q : Queue (BinTree α)) :=
+  SBS (q.front) + SBS (q.back)
+
+def SBQ' {α : Type*} (q : Queue (BinTree α)) :=
+  SBS' (q.front) + SBS' (q.back)
+
+def height {α : Type*} : BinTree α → ℕ
+  | empty      => 0
+  | node _ left right =>
+    1 + max (height left) (height right)
+
+def Bi_to_List_df {α : Type*} : BinTree α → List α
+  | empty => []
+  | node a left right =>
+    Bi_to_List_df left ++ a :: Bi_to_List_df right
+
+theorem size_of_app
+{α : Type*} (s1 s2 : Stack (BinTree α)) :
+SBS (s1.app s2) = SBS s1 + SBS s2 := by
+  induction s1 with
+  | empty =>
+    rw [SBS, Nat.zero_add, Stack.app]
+  | push b q1 h =>
+  rw [Stack.app, SBS, h, SBS,
+      Nat.add_assoc]
+
+theorem size_of_app'
+{α : Type*} (s1 s2 : Stack (BinTree α)) :
+SBS' (s1.app s2) = SBS' s1 + SBS' s2 := by
+  induction s1 with
+  | empty =>
+    rw [SBS', Nat.zero_add, Stack.app]
+  | push b q1 h =>
+    rw [Stack.app, SBS', h, SBS', Nat.add_assoc]
+
+theorem size_of_ptb {α : Type*}
+(a : BinTree α) (s : Stack (BinTree α)) :
+SBS (Stack.ptb a s) = SBS s + size a := by
+  induction s with
+  | empty =>
+    rw [Stack.ptb, SBS, SBS, SBS, Nat.add_zero, Nat.zero_add]
+  | push b s ih =>
+    rw [Stack.ptb, SBS, SBS, ih]; omega
+
+theorem size_of_ptb' {α : Type*}
+(a : BinTree α) (s : Stack (BinTree α)) :
+SBS' (Stack.ptb a s) = SBS' s + size' a := by
+  induction s with
+  | empty =>
+    rw [Stack.ptb, SBS', SBS', SBS',
+        Nat.add_zero, Nat.zero_add]
+  | push b s ih =>
+    rw [Stack.ptb, SBS', SBS', ih]; omega
+
+theorem size_of_rev {α : Type*} (q : Stack (BinTree α)) :
+SBS q.rev_tr = SBS q := by
+  rw [Stack.rev_eq]
+  induction q with
+  | empty =>
+    rw [Stack.rev, SBS]
+  | push a as ih =>
+    rw [SBS, ← ih, Stack.rev, size_of_ptb, Nat.add_comm]
+
+theorem size_of_rev' {α : Type*} (q : Stack (BinTree α)) :
+SBS' q.rev_tr = SBS' q := by
+  rw [Stack.rev_eq]
+  induction q with
+  | empty =>
+    rw [Stack.rev, SBS']
+  | push a as ih =>
+    rw [SBS', ← ih, Stack.rev, size_of_ptb', Nat.add_comm]
+
+theorem size_ne_zero' {α : Type*} (b : BinTree α) :
+size' b ≠ 0 := by
+  cases b with
+  | empty =>
+    rw [size']; tauto
+  | node a l r =>
+    rw [size']
+    simp only [ne_eq, Nat.add_eq_zero, Nat.succ_ne_self,
+               false_and, not_false_eq_true]
+
+theorem SBS_eq_zero_iff_empty' {α : Type*}
+(s : Stack (BinTree α)) :
+SBS' s = 0 ↔ s = Stack.empty := by
+  constructor
+  · intro h
+    cases s with
+    | empty => rfl
+    | push a s =>
+      rw [SBS', Nat.add_eq_zero] at h
+      rcases h with ⟨h, -⟩
+      have h2 := size_ne_zero' a
+      contradiction
+  intro h
+  rw [h, SBS']
+
+def breadthFirstAux {α : Type*} (acc : List α)
+(q : Queue (BinTree α)) :=
+  match h : Queue.dequeue q with
+  | (none, _) => acc
+  | (some a, p) => match a with
+    | empty => breadthFirstAux acc p
+    | node a l r => breadthFirstAux
+        (a :: acc) (Queue.enqueue r (Queue.enqueue l p))
+termination_by SBQ' q
+
+decreasing_by
+  · cases q with
+    | mk front back =>
+      cases front with
+      | empty =>
+        cases back with
+        | empty =>
+          rw [SBQ', SBQ', SBS', Nat.add_zero]
+          rw [Queue.dequeue] at h
+          dsimp at h
+          rw [Stack.rev_tr, Stack.app_rev] at h
+          dsimp at h
+          rw [Prod.mk_inj] at h; tauto
+        | push b back =>
+          nth_rewrite 2 [SBQ']
+          rw [SBS', SBS', Nat.zero_add]
+          rw [Queue.dequeue] at h
+          dsimp at h
+          rw [Stack.rev_eq, Stack.rev] at h
+          have := Stack.exists_push_of_ptb
+            (a := b) (s := back.rev)
+          rcases this with ⟨c, s, h2⟩
+          rw [← h2] at h
+          dsimp at h
+          rw [Prod.mk_inj] at h
+          rcases h with ⟨h3, h4⟩
+          rw [Option.some_inj] at h3
+          rw [← h4, SBQ', SBS', Nat.add_zero]
+          dsimp
+          apply Nat.lt_of_lt_of_le (m := size' c + SBS' s)
+          · rw [Nat.lt_add_left_iff_pos]
+            have h5 := size_ne_zero' c
+            omega
+          have h5 : SBS' (Stack.push c s) =
+            SBS' (Stack.ptb b back.rev) := by rw [h2]
+          rw [SBS', size_of_ptb', ← Stack.rev_eq,
+              size_of_rev'] at h5
+          rw [h5, Nat.add_comm]
+          apply Nat.le_refl
+      | push b front =>
+        rw [Queue.dequeue] at h
+        dsimp at h
+        rw [Prod.mk_inj] at h
+        rcases h with ⟨h1, h2⟩; clear h
+        rw [Option.some_inj] at h1
+        rw [h1, ← h2]; simp only [SBQ', SBS']
+        rw [size']
+        omega
+  rw [Queue.enqueue, Queue.enqueue, SBQ', SBQ']
+  dsimp
+  rw [SBS', SBS']
+  cases q with
+  | mk front back =>
+    cases front with
+    | empty =>
+      cases back with
+      | empty =>
+        rw [Queue.dequeue] at h
+        dsimp at h
+        rw [Stack.rev_tr, Stack.app_rev] at h
+        dsimp at h
+        rw [Prod.mk_inj] at h
+        tauto
+      | push c back =>
+        rw [Queue.dequeue] at h
+        dsimp at h
+        rw [Stack.rev_eq, Stack.rev] at h
+        have h2 := Stack.exists_push_of_ptb (a := c) back.rev
+        rcases h2 with ⟨b, s, h2⟩
+        rw [← h2] at h
+        dsimp at h
+        rw [Prod.mk_inj, Option.some_inj] at h
+        rcases h with ⟨h3, h4⟩; clear h
+        rw [← h4]
+        dsimp
+        rw [SBS', Nat.add_zero, Nat.zero_add, SBS']
+        have h5 : SBS' (Stack.push b s) =
+          SBS' (Stack.ptb c back.rev) := by rw [h2]
+        rw [SBS', size_of_ptb', ← Stack.rev_eq,
+            size_of_rev', h3, size'] at h5
+        rw [Nat.add_comm (n := c.size'), ← h5]
+        omega
+    | push b front =>
+      dsimp
+      rw [Queue.dequeue] at h
+      dsimp at h
+      rw [Prod.mk_inj, Option.some_inj] at h
+      rcases h with ⟨h1, h2⟩; clear h
+      rw [← h2, h1]
+      dsimp
+      rw [SBS', size']
+      omega
+
+def Bi_to_List_bf {α : Type*} : BinTree α → List α
+  | b => List.reverse (breadthFirstAux
+      [] (Queue.enqueue b Queue.empty))
+
+end BinTree
