MyLean/MyDataStructures/test.lean
@@ -1,0 +1,24 @@
+import MyLean.MyDataStructures.BinTree
+
+open BinTree
+
+#eval Queue.mk (Stack.list_to_stack [1, 3, 5]) (Stack.list_to_stack [5, 2, 2])
+
+def mytree1 := BinTree.node 2 (node 3 empty empty) (node 5 empty empty)
+def mytree2 := node 6 (node 8 empty mytree1) (node 7 empty mytree1)
+
+def empty_q := (Queue.empty : Queue (BinTree ℕ))
+
+def myqueue1 := Queue.enqueue mytree1 empty_q
+def myqueue2 := Queue.enqueue mytree2 myqueue1
+
+#eval mytree1
+#eval mytree2
+
+#eval size mytree1
+#eval size mytree2
+#eval size' mytree1
+#eval size' mytree2
+
+#eval Bi_to_List_df mytree2
+#eval Bi_to_List_bf mytree2
